examples/new_echo/NewEcho0.v
@@ -46,7 +46,7 @@ Section PROOF.
     fun args =>
       h <- (pargs [Tuntyped] args)?;;
       `n: val    <- (ccallU "getint" ([]: list val));;
-      assume (wf_val n);;;
+      assume((wf_val n) /\ (match n with | Vint _ => True | _ => False end));;;
       if (dec n (Vint (- 1)))
       then Ret Vundef
       else
@@ -66,7 +66,7 @@ Section PROOF.
     fun args =>
       h <- (pargs [Tuntyped] args)?;;
       `n: val    <- (ccallU "pop" ([h]: list val));;
-      assume (wf_val n);;;
+      assume((wf_val n) /\ (match n with | Vint _ => True | _ => False end));;;
       if (dec n (Vint (- 1)))
       then Ret Vundef
       else
